add partial correctness hoare triples

deps/coq-poulet4/lib/Monads/Hoare/WP.v
@@ -22,47 +22,59 @@ Definition bot {State: Type} : Pred State := fun _ => False.
 Hint Unfold top : core.
 Hint Unfold bot: core.
 
-Definition hoare_triple_wp
-    {State Exception Result: Type}
-    {P: Pred State}
-    {c: @state_monad State Exception Result}
-    {Q: Post State (Result + Exception)}
+
+Definition hoare_total_wp
+  {State Exception Result: Type}
+  {P: Pred State}
+  {c: @state_monad State Exception Result}
+  {Q: Post State (Result + Exception)}
     : Prop := 
   forall st, P st -> 
   let (v, st') := c st in
     Q v st'.
 
-Definition Norm {A State Exception} (f: A -> State -> Prop) : Post State (A + Exception) := fun r s => 
-  match r with 
-  | inl v => f v s
+Notation "{{ P }} c {{ Q }}" := (@hoare_total_wp _ _ _ P c Q) (at level 90) : hoare_scope_wp.
+
+Definition hoare_partial_wp
+  {State Exception Result: Type}
+  {P: Pred State}
+  {c: @state_monad State Exception Result}
+  {Q: Post State Result}
+    : Prop := 
+  forall st, P st -> 
+  let (v, st') := c st in
+  match v with 
+  | inl r => Q r st'
   | inr _ => False
   end.
 
+Notation "<< P >> c << Q >>" := (@hoare_partial_wp _ _ _ P c Q) (at level 90) : hoare_scope_wp.
 
-Notation "{{ P }} c {{ Q }}" := (@hoare_triple_wp _ _ _ P c Q) (at level 90) : hoare_scope_wp.
+
 Ltac mysimp := 
-    unfold Pred, Post, hoare_triple_wp, state_return, state_bind, get_state, put_state in * ; intros ; 
-      repeat (match goal with
-                | [ H : ?P |- ?P ] => exact H
-                | [ H : _ /\ _ |- _] => destruct H
-                | [ H : (_ * _)%type |- _] => destruct H
-                | [ H : (_ + _)%type |- _] => destruct H
-                | [ H1 : forall _, ?P1 _ -> _, H2 : ?P1 ?h |- _] => 
-                  generalize (H1 h H2) ; clear H1 ; intros
-                | [ H1 : forall _ _ _, ?P1 _ _ -> _, H2 : ?P1 ?x ?h |- _] => 
-                  generalize (H1 _ _ _ H2) ; clear H1 ; intros
-                | [ H : match ?e with | Some _ => _ | None => _ end |- _ ] => 
-                  destruct e
-                | [ |- _ /\ _ ] => split
-                | [ H : exists _, _ |- _] => destruct H
-                | [ H : Some ?x = Some ?y |- _ ] => inversion H ; clear H ; subst
-                | [ H : inl ?x = inl ?y |- _ ] => inversion H ; clear H ; subst
-                | [ H : inr ?x = inr ?y |- _ ] => inversion H ; clear H ; subst
-                | _ => assert False ; [ lia | contradiction ]
-              end) ; subst ; simpl in * ; try firstorder ; auto with arith.
+  unfold Pred, Post, hoare_total_wp, hoare_partial_wp, state_return, state_bind, get_state, put_state in * ; intros ; 
+  repeat (
+    match goal with
+    | [ H : ?P |- ?P ] => exact H
+    | [ H : _ /\ _ |- _] => destruct H
+    | [ H : (_ * _)%type |- _] => destruct H
+    | [ H : (_ + _)%type |- _] => destruct H
+    | [ H1 : forall _, ?P1 _ -> _, H2 : ?P1 ?h |- _] => 
+      generalize (H1 h H2) ; clear H1 ; intros
+    | [ H1 : forall _ _ _, ?P1 _ _ -> _, H2 : ?P1 ?x ?h |- _] => 
+      generalize (H1 _ _ _ H2) ; clear H1 ; intros
+    | [ H : match ?e with | Some _ => _ | None => _ end |- _ ] => 
+      destruct e
+    | [ |- _ /\ _ ] => split
+    | [ H : exists _, _ |- _] => destruct H
+    | [ H : Some ?x = Some ?y |- _ ] => inversion H ; clear H ; subst
+    | [ H : inl ?x = inl ?y |- _ ] => inversion H ; clear H ; subst
+    | [ H : inr ?x = inr ?y |- _ ] => inversion H ; clear H ; subst
+    | _ => assert False ; [ lia | contradiction ]
+    end) ; subst ; simpl in * ; try firstorder ; auto with arith.
 
 
-Lemma strengthen_pre
+Lemma strengthen_pre_t
   {State Exception Result:Type} 
   {P1: Pred State} 
   {P2: Pred State}
@@ -76,7 +88,21 @@ Proof.
   mysimp.
 Qed.
 
-Lemma return_wp {State Exception Result: Type} 
+Lemma strengthen_pre_p
+  {State Exception Result:Type} 
+  {P1: Pred State} 
+  {P2: Pred State}
+  {c: @state_monad State Exception Result}
+  {Q : Post State Result} 
+  :
+  << P1 >> c << Q >> ->
+  (forall h, P2 h -> P1 h) ->
+  << P2 >> c << Q >>.
+Proof.
+  mysimp.
+Qed.
+
+Lemma return_wp_t {State Exception Result: Type} 
   {Q: Post State (Result + Exception)} 
   (x: Result) : 
   {{ Q (inl x) }} 
@@ -86,7 +112,18 @@ Proof.
   mysimp.
 Qed.
 
-Lemma fail_wp {State Exception Result: Type} 
+Lemma return_wp_p {State Exception Result: Type} 
+  {Q: Post State Result} 
+  (x: Result) : 
+  << Q x >> 
+    @state_return State Exception Result x 
+  << Q >>.
+Proof.
+  mysimp.
+Qed.
+
+
+Lemma fail_wp_t {State Exception Result: Type} 
   {Q: Post State (Result + Exception)}
   (e: Exception) : 
   {{ Q (inr e)}} 
@@ -96,7 +133,17 @@ Proof.
   mysimp.
 Qed.
 
-Lemma get_wp {State Exception: Type} 
+Lemma fail_wp_p {State Exception Result: Type} 
+  {Q: Post State Result}
+  (e: Exception) : 
+  << bot >> 
+    @state_fail State Exception Result e 
+  << Q >>.
+Proof.
+  mysimp.
+Qed.
+
+Lemma get_wp_t {State Exception: Type} 
   {Q: Post State (State + Exception)}
   :
   {{ fun s => Q (inl s) s }} 
@@ -106,7 +153,17 @@ Proof.
   mysimp.
 Qed.
 
-Lemma put_wp {State Exception Result: Type} 
+Lemma get_wp_p {State Exception: Type} 
+  {Q: Post State State }
+  :
+  << fun s => Q s s >> 
+    @get_state State Exception 
+  << Q >>.
+Proof.
+  mysimp.
+Qed.
+
+Lemma put_wp_t {State Exception: Type} 
   {Q: Post State (unit + Exception)}  
   f :
   {{ fun s => Q (inl tt) (f s) }} 
@@ -116,7 +173,17 @@ Proof.
   mysimp.
 Qed.
 
-Lemma bind_wp
+Lemma put_wp_p {State Exception: Type} 
+  {Q: Post State unit}  
+  f :
+  << fun s => Q tt (f s) >> 
+    @put_state State Exception f 
+  << Q >>.
+Proof.
+  mysimp.
+Qed.
+
+Lemma bind_wp_t
   {State A B Exception: Type}
   {P: Pred State}
   {Pa: A -> Pred State}
@@ -146,7 +213,29 @@ Proof.
       trivial.
 Qed.
 
-Lemma cond_wp
+Lemma bind_wp_p
+  {State A B Exception: Type}
+  {P: Pred State}
+  {P': Post State A}
+  {Q: Post State B}
+  {c: @state_monad State Exception A}
+  {f: A -> @state_monad State Exception B}
+  :
+  << P >> c << P' >> ->
+  (forall r: A, << P' r >> (f r) << Q >>) -> 
+  << P >> c >>= f << Q >>.
+Proof.
+  intros.
+  mysimp.
+  mysimp.
+  destruct (c st).
+  destruct s.
+    - eapply H0.  
+      trivial.
+    - trivial.
+Qed.
+
+Lemma cond_wp_t
   {State Exception Result: Type} 
   {b: bool}
   {P1 P2 Q} 
@@ -161,7 +250,22 @@ Proof.
   destruct b; mysimp.
 Qed.
 
-Lemma case_nat_wp
+Lemma cond_wp_p
+  {State Exception Result: Type} 
+  {b: bool}
+  {P1 P2 Q} 
+  {c1 c2 : @state_monad State Exception Result}: 
+  << P1 >> c1 << Q >> ->
+  << P2 >> c2 << Q >> ->
+  << fun s => if b then P1 s else P2 s >> 
+    if b then c1 else c2 
+  << Q >>.
+Proof.
+  intros.
+  destruct b; mysimp.
+Qed.
+
+Lemma case_nat_wp_t
   {State Exception Result: Type} 
   {P1 P2 Q c1} 
   {c2: nat -> @state_monad State Exception Result} n : 
@@ -186,6 +290,31 @@ Proof.
   destruct n; mysimp.
 Qed.
 
+Lemma case_nat_wp_p
+  {State Exception Result: Type} 
+  {P1 P2 Q c1} 
+  {c2: nat -> @state_monad State Exception Result} n : 
+  << fun s => P1 s /\ n = 0 >> c1 << Q >> ->
+  << fun s => exists n', n = S n' /\ P2 n' s >> 
+    (c2 (Nat.pred n)) 
+  << Q >> ->
+  << 
+    match n with 
+    | 0 => P1
+    | S n' => P2 n' 
+    end
+  >>
+    match n with 
+    | 0 => c1 
+    | S n' => c2 n'
+    end
+  <<
+    Q
+  >>.
+Proof.
+  destruct n; mysimp.
+Qed.
+
 Definition destruct_list' {A} (xs: list A) (default: A) : A * list A := 
   match xs with
   | nil => (default, nil)
@@ -193,7 +322,7 @@ Definition destruct_list' {A} (xs: list A) (default: A) : A * list A :=
   end.
 
 
-Lemma case_list_wp
+Lemma case_list_wp_t
   {State Exception Result A: Type} 
   {P1 P2 Q c1} 
   {dummy: A }
@@ -219,13 +348,39 @@ Proof.
   destruct xs; mysimp.
 Qed.
 
+Lemma case_list_wp_p
+  {State Exception Result A: Type} 
+  {P1 P2 Q c1} 
+  {dummy: A }
+  {c2: A -> list A -> @state_monad State Exception Result} xs : 
+  << fun s => P1 s /\ xs = nil >> c1 << Q >> ->
+  << fun s => exists x xs', xs = x :: xs' /\ P2 x xs' s >> 
+    (c2 (fst (destruct_list' xs dummy)) (snd (destruct_list' xs dummy))) 
+  << Q >> ->
+  << 
+    match xs with 
+    | nil => P1
+    | x :: xs' => P2 x xs' 
+    end
+  >>
+    match xs with 
+    | nil => c1 
+    | x :: xs' => c2 x xs'
+    end
+  <<
+    Q
+  >>.
+Proof.
+  destruct xs; mysimp.
+Qed.
+
 Definition destruct_opt {A} (opt: option A) (dummy: A) :=
   match opt with
   | Some x => x
   | None => dummy
   end.
 
-Lemma case_option_wp
+Lemma case_option_wp_t
   {State Exception Result A: Type} 
   {P1 P2 Q c1} 
   {dummy: A}
@@ -251,7 +406,33 @@ Proof.
   destruct x; mysimp.
 Qed.
 
-Lemma hoare_consequence
+Lemma case_option_wp_p
+  {State Exception Result A: Type} 
+  {P1 P2 Q c1} 
+  {dummy: A}
+  {c2: A -> @state_monad State Exception Result} x : 
+  << fun s => P1 s /\ x = None >> c1 << Q >> ->
+  << fun s => exists x', x = Some x' /\ P2 x' s >> 
+    (c2 (destruct_opt x dummy)) 
+  << Q >> ->
+  << 
+    match x with 
+    | None => P1
+    | Some x' => P2 x' 
+    end
+  >>
+    match x with 
+    | None => c1
+    | Some x' => c2 x'
+    end
+  <<
+    Q
+  >>.
+Proof.
+  destruct x; mysimp.
+Qed.
+
+Lemma hoare_consequence_t
   {State Exception Result:Type} 
   {P1: Pred State} 
   {P2: Pred State}
@@ -269,7 +450,25 @@ Proof.
   mysimp.
 Qed.
 
-Lemma weaken_post
+Lemma hoare_consequence_p
+  {State Exception Result:Type} 
+  {P1: Pred State} 
+  {P2: Pred State}
+  {Q1: Post State Result}
+  {Q2: Post State Result}
+  {c: @state_monad State Exception Result}
+  :
+  << P1 >> c << Q1 >> ->
+  (forall h, P2 h -> P1 h) ->
+  (forall v h, Q1 v h -> Q2 v h) ->
+  << P2 >> c << Q2 >>.
+Proof.
+  mysimp.
+  destruct (c st).
+  mysimp.
+Qed.
+
+Lemma weaken_post_t
   {State Exception Result:Type} 
   {P: Pred State} 
   {Q1: Post State (Result + Exception)}
@@ -280,7 +479,24 @@ Lemma weaken_post
   {{ P }} c {{ Q2 }}.
 Proof.
   intros.
-  apply (hoare_consequence H).
+  apply (hoare_consequence_t H).
+  mysimp.
+  intros.
+  apply H0; trivial.
+Qed.
+
+Lemma weaken_post_p
+  {State Exception Result:Type} 
+  {P: Pred State} 
+  {Q1: Post State Result}
+  {Q2: Post State Result}
+  {c: @state_monad State Exception Result} :
+  << P >> c << Q1 >> -> 
+  (forall v s, Q1 v s -> Q2 v s) ->
+  << P >> c << Q2 >>.
+Proof.
+  intros.
+  apply (hoare_consequence_p H).
   mysimp.
   intros.
   apply H0; trivial.
@@ -288,13 +504,49 @@ Qed.
 
 Ltac wp :=
   match goal with
-  | [ |- {{ _ }} mbind _ _ {{ _ }} ] => eapply bind_wp
-  | [ |- {{ _ }} get_state {{ _ }} ] => eapply get_wp
-  | [ |- {{ _ }} put_state ?e {{ _ }} ] => eapply (put_wp e)
-  | [ |- {{ _ }} state_fail ?e {{ _ }} ] => eapply (fail_wp e)
-  | [ |- {{ _ }} state_return ?e {{ _ }} ] => eapply (return_wp e)
-  | [ |- {{ _ }} if _ then _ else _ {{ _ }} ] => eapply cond_wp
-  | [ |- {{ _ }} match ?e with | 0 => _ | S _ => _ end {{ _ }} ] => eapply (case_nat_wp e)
-  | [ |- {{ _ }} match ?e with | nil => _ | _ :: _ => _ end {{ _ }} ] => eapply (case_list_wp e)
-  | [ |- {{ _ }} match ?e with | Some _ => _ | None => _ end {{ _ }} ] => eapply (case_option_wp e)
+  | [ |- {{ _ }} mbind _ _ {{ _ }} ] => eapply bind_wp_t
+  | [ |- {{ _ }} get_state {{ _ }} ] => eapply get_wp_t
+  | [ |- {{ _ }} put_state ?e {{ _ }} ] => eapply (put_wp_t e)
+  | [ |- {{ _ }} state_fail ?e {{ _ }} ] => eapply (fail_wp_t e)
+  | [ |- {{ _ }} state_return ?e {{ _ }} ] => eapply (return_wp_t e)
+  | [ |- {{ _ }} if _ then _ else _ {{ _ }} ] => eapply cond_wp_t
+  | [ |- {{ _ }} match ?e with | 0 => _ | S _ => _ end {{ _ }} ] => eapply (case_nat_wp_t e)
+  | [ |- {{ _ }} match ?e with | nil => _ | _ :: _ => _ end {{ _ }} ] => eapply (case_list_wp_t e)
+  | [ |- {{ _ }} match ?e with | Some _ => _ | None => _ end {{ _ }} ] => eapply (case_option_wp_t e)
+  | [ |- << _ >> mbind _ _ << _ >> ] => eapply bind_wp_p
+  | [ |- << _ >> get_state << _ >> ] => eapply get_wp_p
+  | [ |- << _ >> put_state ?e << _ >> ] => eapply (put_wp_p e)
+  | [ |- << _ >> state_fail ?e << _ >> ] => eapply (fail_wp_p e)
+  | [ |- << _ >> state_return ?e << _ >> ] => eapply (return_wp_p e)
+  | [ |- << _ >> if _ then _ else _ << _ >> ] => eapply cond_wp_p
+  | [ |- << _ >> match ?e with | 0 => _ | S _ => _ end << _ >> ] => eapply (case_nat_wp_p e)
+  | [ |- << _ >> match ?e with | nil => _ | _ :: _ => _ end << _ >> ] => eapply (case_list_wp_p e)
+  | [ |- << _ >> match ?e with | Some _ => _ | None => _ end << _ >> ] => eapply (case_option_wp_p e)
   end.
+
+
+Definition Norm {A State Exception} (f: A -> State -> Prop) : Post State (A + Exception) := fun r s => 
+  match r with 
+  | inl v => f v s
+  | inr _ => False
+end.
+
+Lemma lift_partial {State Exception Result: Type}:
+  forall (P: Pred State) (c: @state_monad State Exception Result) (Q: Post State Result),
+  << P >> c << Q >> ->
+  {{ P }} c {{ Norm Q }}.
+Proof.
+  mysimp.
+Qed.
+
+(* It turns out that hoare triples over a monad form a monad as well! Using this insight,
+   we can automate much of the intermediate plumbing for partial correctness proofs. 
+   The notation below allows for building such proofs; see examples/Hoare.v for usage.
+
+   Alas, the dual postconditions for total correctness seem to preclude similar plumbing
+   for total correctness proofs. 
+ *)
+Notation "x <-- c ; f" := (bind_wp_p c (fun x => f))
+  (right associativity, at level 84, c at next level) : hoare_scope_wp.
+Notation "c ;;; f" := (bind_wp_p c (fun _:unit => f))
+  (right associativity, at level 84) : hoare_scope_wp.
