deps/coq-poulet4/examples/Hoare.v
@@ -6,68 +6,76 @@ Require Import Lia.
 Require Import Coq.Init.Nat.
 Require Import Coq.Lists.List.
 
+(* Using the WP hoare calculus, we can reason about output states and results for monadic programs.
+   
+  To reason about programs that might fail under a precondition P, we must use a total hoare calculus, notated by: 
+    {{ P }} potentially_failing_program {{ Q }}.
+    For such programs Q must handle both the normal and error cases, and so is a function 
+    (Result + Exception) -> State -> Prop.
 
-Definition either_or (n: nat): @state_monad nat unit bool := 
-  match n with 
-  | 0 => state_return true
-  | S n' => put_state (fun _ => 0) ;; state_fail tt
-  end.
-  
-Example get_incr n:
-  {{ fun s => s = n  }}
-    @put_state nat unit (fun x => x + 1) ;; @get_state nat unit
-  {{ Norm (fun r s => r = n + 1) }}.
-Proof.
-  eapply bind_wp.
-  all: swap 2 1.
-  intros. 
-  eapply get_wp.
-  all: swap 2 1.
-  intros.
-  apply H.
-  mysimp.
-Qed.
+  While this total calculus is expressive, it's convenient to restrict the scope to
+  partial triples, in which the program will never fail under a precondition P.
+  For this we notate a partial hoare triple as 
+  << P >> always_successful_program << Q >>.
 
+  A benefit of partial triples is that we can use the monadic properties of the specification calculus
+  to automate proofs. See the bottom of this file for examples.
+*)
 
+(* Consider a silly program with a single nat as state, that increments the nat and
+ * immediately fails. We can prove that this program A) always fails and B) increments the state.
+ *)
 Example fail_incr n:
   {{ fun s => s = n }}
     @put_state nat unit (fun x => x + 1) ;; @state_fail nat unit nat tt
   {{ fun ve s => 
     match ve with 
-    | inl _ => False
-    | inr _ => s = n + 1
+    | inl _ => False (* property A), the program always fails *)
+    | inr _ => s = n + 1 (* property B), the final state is one larger than the initial state *)
     end
   }}.
 Proof.
-  eapply bind_wp.
+  wp.
   all: swap 2 1. 
   intros.
-  eapply strengthen_pre.
-  eapply fail_wp.
+  eapply strengthen_pre_t.
+  wp.
   intros.
   simpl.
   apply H.
   all: swap 2 1.
   intros.
   apply H.
-
-
-  eapply strengthen_pre.
-  eapply put_wp.
+  
+  eapply strengthen_pre_t.
+  wp.
   mysimp.
   Unshelve.
   exact unit.
 Qed.
 
+(* Similarly, consider a program that checks a condition and fails if the condition is true.
+   We can prove that this program will always fail if the condition is true.
+*)
 Example cond_fail b:
   {{ fun s => s = b /\ b = true }}
     if b then state_fail tt else state_return true
   {{ fun r s => r = inr tt }}.
 Proof.
-  eapply strengthen_pre.
+  eapply strengthen_pre_t.
   repeat wp.
   mysimp.
 Qed.
+
+(* Another interesting program is one that can either succeed or fail, and on failure cases,
+ * always sets the state to 0. We can prove that either it succeeded or the state is always 0.
+ *)
+Definition either_or (n: nat): @state_monad nat unit bool := 
+  match n with 
+  | 0 => state_return true
+  | S n' => put_state (fun _ => 0) ;; state_fail tt
+  end.
+
 Example eo_pres n:
   {{ top }}
     either_or n
@@ -79,23 +87,23 @@ Example eo_pres n:
   }}.
 Proof.
   unfold either_or.
-  eapply strengthen_pre.
-  eapply (case_nat_wp n).
-  eapply strengthen_pre.
-  eapply return_wp.
+  eapply strengthen_pre_t.
+  wp.
+  eapply strengthen_pre_t.
+  wp.
   intros.
   destruct H as [it _].
   exact it.
 
-  eapply strengthen_pre.
-  eapply bind_wp.
+  eapply strengthen_pre_t.
+  wp.
   all: swap 2 1.
   intros.
-  eapply strengthen_pre.
-  eapply fail_wp.
+  eapply strengthen_pre_t.
+  wp.
   intros.
   exact H.
-  eapply put_wp.
+  wp.
   intros.
   simpl.
   exact H.
@@ -109,45 +117,11 @@ Proof.
   exact unit.
 Qed.
 
-Example eo_pres' n:
-  {{ top }}
-    either_or n
-  {{ fun r s => 
-    match r with 
-    | inl r' => r' = true
-    | inr _  => s = 0
-    end
-  }}.
-Proof.
-  unfold either_or.
-  eapply strengthen_pre.
-  wp.
-  eapply strengthen_pre.
-  wp.
 
-  intros.
-  destruct H as [it _].
-  exact it.
-
-  wp.
-  all: swap 2 1.
-  intros.
-  eapply strengthen_pre.
-  wp.
-  intros.
-  exact H.
-  eapply strengthen_pre.
-  wp.
-  intros.
-  destruct H as [n' [eq it]].
-  exact it.
-  intros.
-  exact H.
-  destruct n; mysimp.
-  Unshelve.
-  exact unit.
-Qed.
-
+(* We can also combine the either_or program with a function that reads the state,
+ * and prove the same postcondition. We can further leverage the proof of either_or
+ * halfway through the proof.
+ *)
 Definition get_branch : @state_monad nat unit bool := 
   n <- get_state ;; either_or n.
 
@@ -161,18 +135,24 @@ Example branch_splits :
     end
    }}.
 Proof.
-  eapply strengthen_pre.
+  eapply strengthen_pre_t.
   unfold get_branch.
   wp.
   all: swap 2 1.
 
   intros.
-  apply (eo_pres r).
+  apply (eo_pres r). (* reuse a prior proof *)
   wp.
   intros.
   exact H.
   mysimp.
 Qed.
+
+(* While our hoare calculi do not have primitives for loops, we can still easily
+ * prove properties about left-folds using Coq's induction tactic. 
+ * Consider a function that takes an input n and increments a state n times.
+ * We can prove that it correctly performs the addition.
+ *)
 
 Fixpoint iter_incr (n: nat) : @state_monad nat unit unit :=
   match n with 
@@ -180,21 +160,21 @@ Fixpoint iter_incr (n: nat) : @state_monad nat unit unit :=
   | S n' => iter_incr n' ;; put_state (fun x => x + 1)
   end.
 
-Lemma iter_incr_n n m:
+Example iter_incr_t n m:
   {{ fun s => s = n }}
     iter_incr m
-  {{ Norm (fun r s' => s' = n + m )}}.
+  {{ Norm (fun r s' => s' = n + m )}}. (* the function does not error and adds the numbers *)
 Proof.
   induction m.
   - unfold iter_incr.
     mysimp.
   - unfold iter_incr. fold iter_incr.
-    eapply strengthen_pre.
+    eapply strengthen_pre_t.
     wp.
     all: swap 2 1.
     intros. 
     wp.
-    eapply weaken_post.
+    eapply weaken_post_t.
     apply IHm.
     all: swap 2 1.
     intros.
@@ -205,4 +185,85 @@ Proof.
   Unshelve.
   exact unit.
 Qed.
+
   
+(* While the proofs before were not painful, there is still room for automation.
+ * Consider a function that increments the state and then immediatly gets the state.
+ * In total correctness, we can prove the returned value is one larger than the  
+ * input state using two applications of bind.
+ *)
+
+Example get_incr_t n:
+  {{ fun s => s = n  }}
+    @put_state nat unit (fun x => x + 1) ;; @get_state nat unit
+  {{ Norm (fun r s => r = n + 1) }}.
+Proof.
+  wp.
+  all: swap 2 1.
+  intros. 
+  wp.
+  all: swap 2 1.
+  intros.
+  apply H.
+  mysimp.
+Qed.
+
+(* Notice that this function never fails, so we can use the partial calculus as well.
+ * With the partial calculus we can use the monadic proof combinators and build
+ * a proof skeleton using refine and strengthen_pre_p for a substantially shorter proof.
+ * C
+ *)
+
+Example get_incr_p n:
+  << fun s => s = n  >>
+    @put_state nat unit (fun x => x + 1) ;; @get_state nat unit
+  << fun r s => r = n + 1 >>.
+Proof.
+  refine (strengthen_pre_p ( 
+    @put_wp_p nat unit _ (fun x => x + 1) ;;; @get_wp_p nat unit _
+  ) _). 
+  (* Notice that Coq filled in the details of bind and so we are left to prove that 
+     our specific precondition actually entails the weakest precondition.
+     (spoiler: it does, because we gave a logically equivalent precondition ) 
+  *)
+  mysimp.
+Qed.
+
+(* The conditional fail example from before can be similarly automated. *)
+
+Example cond_fail_p b:
+  << fun s => s = b /\ b = false >>
+    if b then state_fail tt else state_return true
+  << fun r s => r = true >>.
+Proof.
+  refine (strengthen_pre_p ( 
+    cond_wp_p (fail_wp_p tt) (return_wp_p true)
+  ) _).
+  mysimp.
+Qed.
+
+(* But what about loops? It's a bit more subtle here, but we can in fact use the same technique. *)
+
+Example iter_incr_n_p n m:
+  << fun s => s = n >>
+    iter_incr m
+  << fun _ s' => s' = n + m >>.
+Proof.
+  induction m.
+
+  (* The base case is as before. *)
+  - unfold iter_incr.
+    mysimp.
+
+  (* In the recursive case, the question becomes "what to put as the first triple in the hoare proof?"
+   * A natural fit is the inductive hypothesis! It almost works, but the post condition needs
+   * to be massaged to align with the weakest-precondition of the final state update.
+   * So to do this, we wrap the inductive hypothesis with weaken_post_p.
+   *)
+  - unfold iter_incr. fold iter_incr.
+    refine (strengthen_pre_p (
+      weaken_post_p IHm _ ;;; put_wp_p (fun x => x + 1)
+    ) _);
+    (* viola! and we are left with some trivial math constraints. *)
+    lia.
+Qed.
